extra/LambdaExtra.v
@@ -5063,3 +5063,4 @@ Proof using. (* might be simplified using rule_for_trm *)
     lets: hpure_inv Z. false*. } (* LATER: shorten *)
 Qed.
 
+
